{
 "cells": [
  {
   "cell_type": "markdown",
   "metadata": {},
   "source": [
    "## Informal Introduction\n",
    "\n",
    "Let say we have series of \\\\(x\\\\), such that:\n",
    "\n",
    "$$x^0, x^1, x^2, ..., x^n, ...$$\n",
    "\n",
    "Each x in the *power series* above has a *coefficient* \\\\(s\\\\), so that the **coefficients of the power series** are:\n",
    "\n",
    "$$s_0, s_1, s_2, ..., s_n, ...$$\n",
    "\n",
    "So, we can conclude that there is a correlation of \\\\(s_i \\rightarrow x^i\\\\)\n",
    "\n",
    "The generating function has main advantage is the power series is a form of **rational number**. For example:\n",
    "\n",
    "$$\\frac{1}{1-x} = 1 + x + x^2 + x^3 + ...$$\n",
    "\n",
    "has the form with exist *multiplier coefficients* such that:\n",
    "\n",
    "$$\\frac{1}{1-x} = s_0 1 + s_1 x + s_2 x^2 + s_3 x^3 + ...$$\n",
    "\n",
    "which is the series of coeffiecients:\n",
    "\n",
    "$$S = 1, 1, 1, 1, ...$$\n",
    "\n",
    "So, the series \\\\(S\\\\) has generating function (GF) \\\\(\\frac{1}{1-x}\\\\)\n",
    "\n",
    "----\n",
    "\n",
    "Another example:\n",
    "\n",
    "$$\\frac{1}{{(1-x)}^2} = 1 + 2x + 3x^2 + 4x^2 + ...$$\n",
    "\n",
    "So, the series of natural number \\\\(1, 2, 3, 4, ...\\\\) has generating function \\\\(\\frac{1}{(1-x)^2}\\\\)\n",
    "\n",
    "\n",
    "## The Relationship Between GF and Recurrence\n",
    "\n",
    "Natural numbers : \\\\(\\{1, 2, 3, 4, ...\\}\\\\) has GF \\\\(\\frac{1}{(1-x)^2} = \\frac{1}{1-2x-x^2}\\\\) and has recurrence \\\\(S_n = 2S{n-1}-S_{n-2}\\\\).\n",
    "\n",
    "We can see that relationship more clearly if we rewrite the recurrence in this form:\n",
    "\n",
    "$$S_n - 2S_{n-1} + S_{n-2} = 0$$\n",
    "\n",
    "And compute that with the denominator of the GF, namely:\n",
    "\n",
    "$$1-2x+X^2$$\n",
    "\n",
    "\n",
    "## Motivation\n",
    "\n",
    "We normally are interested not just in counting combinatorial structures, but also in analyzing their properties. We look at how to use **bivarite** generative functions for this purpose, and how this relates to the use of **probability** generating functions.\n",
    "\n",
    "\n",
    "## Power Series\n",
    "\n",
    "Before jump into the Ordinary Generating Function (OGF), lets take a refershness with the concept of power series. In mathematics, a power series (in one variable) is an infinite series of the form:\n",
    "\n",
    "$$\\sum_{n=0}^\\infty a_n(x-c)^n = a_0 + a_1(x-c)^1 + a_2(x-c)^2 + ... $$\n",
    "\n",
    "where \\\\(a_n\\\\) represents the coefficient of the *n*th term and *c* is a constant. \\\\(a_n\\\\) is independent of *x* and may be expressed as a function of *n* (e.g //(a_n = \\frac{1}{n!}//)). This series usually arise as the **Taylor series** of some known function.\n",
    "\n",
    "In many situasions *c* (the *center* of the series) is equal to zero, for instance when considering a **Maclaurin series**. In such case, the power series takes the simpler form:\n",
    "\n",
    "$$\\sum_{n=0}^\\infty a_n x^n = a_0 + a_1x + a_2x^2 + ...$$\n",
    "\n",
    "\n",
    "### Examples\n",
    "\n",
    "Polynomial function:\n",
    "\n",
    "$$f(x) = x^2 + 2x + 3$$\n",
    "\n",
    "can be expressed as a power series around the center *c* = 0:\n",
    "\n",
    "$$f(x) = 3 + 2x + 1x^2 + 0x^3 + 0x^4 + ... $$\n",
    "\n",
    "or around the center *c* = 1 as:\n",
    "\n",
    "$$f(x) = 6 + 4(x-1) + 1(x-1)^2 + 0(x-1)^3 + 0(x-1)^4 + ...$$\n",
    "\n",
    "So, one can view that power series as being like **polynomials of infinite degree**, altough power series are not polynomials.\n",
    "\n",
    "---\n",
    "\n",
    "The geometric series formula:\n",
    "\n",
    "$$\\frac{1}{1-x} = \\sum_{n=0}{\\infty} x^n = 1 + x + x^2 + x^3 + ..., $$\n",
    "\n",
    "which is valid for \\\\(|x| < 1\\\\), is one of the most important examples of a power series, as are the exponential function formula:\n",
    "\n",
    "$$e^x = \\sum_{n=0}^{\\infty} \\frac{x^n}{n!} = 1 + x + \\frac{x^2}{2!} + \\frac{x^3}{3!} + ...,$$\n",
    "\n",
    "and the sine formula:\n",
    "\n",
    "$$sin(x) = \\sum_{n=0}^{\\infty} \\frac{(-1)^n x^{2n+1}}{(2n+1)!} = x - \\frac{x^3}{3!} + \\frac{x^5}{5!} - \\frac{x^7}{7!} + ...,$$\n",
    "\n",
    "valid for all real x. This power series are also examples of **Taylor series**.\n",
    "\n",
    "\n",
    "## Ordinary Generating Function (OGF)\n",
    "\n",
    "**Definition** Given a sequence \\\\(a_0, a_1, a_2, ..., a_k, ...\\\\), the function\n",
    "\n",
    "$$A(z) = \\sum_{k \\geq 0} a_k z^k$$\n",
    "\n",
    "is called the *Ordinary Generating Function (OGF)* of the sequence. We used notation the notation \\\\(\\lfloor z^k \\rfloor A(z)\\\\) to refer to the coefficuent \\\\(a_k\\\\).\n",
    "\n",
    "Given generating functions \\\\(A(z) = \\sum_{k \\geq 0} a_k z^k\\\\) and \\\\(B(z) = \\sum_{k \\geq 0} b_k z^k\\\\) that represent the sequence \\\\(\\{a_0, a_1, ..., a_k, ...\\}\\\\) and \\\\(\\{b_0, b_1, ... , b_k, ...\\}\\\\), respectively, we can perform a number of simple transformations to get generating functions for other sequences. Several such operations are show is Table 2. Example of the apllication of these operations may be found in the relationships among the entries in Table 1 which are **valid for |z|<1**.\n",
    "\n",
    "| OGF   | Sequence  |                                    \n",
    "|:-----:|:----------|\n",
    "| \\\\(\\sum_{N \\geq 0} z^N = \\frac{1}{1-z}\\\\) | \\\\(1, 1, 1, , ..., 1, ...\\\\) |                                            \n",
    "| \\\\(\\sum_{N \\geq 1} N z^N = \\frac{z}{(1-z)^2}\\\\) | \\\\(0, 1, 2, 3, 4, ..., N, ...\\\\) |                                          \n",
    "| \\\\(\\sum_{N \\geq 2} {N \\choose 2} z^N = \\frac{z^2}{(1-z)^3}\\\\) | \\\\(0, 0, 1, 3, 6, 10, ..., {N \\choose 2}\\\\) |                                        \n",
    "| \\\\(\\sum_{N \\geq M} {N \\choose M} z^N = \\frac{z^M}{(1-z)^{M+1}}\\\\) | \\\\(0, ..., 0, 1 , M+1, ..., {N \\choose M}\\\\) |\n",
    "| \\\\(\\sum_{N \\geq 0}{M \\choose N} z^N = (1+z)^M\\\\) | \\\\(1, M + 1, {M \\choose 2} ..., (M \\choose N), ..., M, 1\\\\) |\n",
    "| \\\\(\\sum_{N \\geq 0} {N+M \\choose N} z^N = \\frac{1}{(1-z)^{M+1}}\\\\) | \\\\(1, M+1, {M+2 \\choose 2}, {M+3 \\choose 3}, ...\\\\) |\n",
    "| \\\\(\\sum_{N \\geq 0} z^{2N} = \\frac{1}{1-z^2}\\\\) | \\\\(1, 0, 1, 0, ..., 1, 0, ...\\\\) |\n",
    "| \\\\(\\sum_{N \\geq 0} c^N z^N = \\frac{1}{1-cz}\\\\) | \\\\(1, c, c^2, c^3, ..., c^N, ...\\\\) |\n",
    "| \\\\(\\sum_{N \\geq 0} \\frac{z^N}{N!} = e^z\\\\) | \\\\(1, 1, \\frac{1}{2!}, \\frac{1}{3!}, \\frac{1}{4!}, ..., \\frac{1}{N!}, ...\\\\) |\n",
    "| \\\\(\\sum_{N \\geq 1} \\frac{z^N}{N} = ln\\frac{1}{1-z}\\\\) | \\\\(0, 1, \\frac{1}{2}, \\frac{1}{3}, \\frac{1}{4}, ..., \\frac{1}{N}, ...\\\\) |\n",
    "| \\\\(\\sum_{N \\geq 1} H_N z^N = \\frac{1}{1-z}ln\\frac{1}{1-z}\\\\) | \\\\(0, 1, 1 + \\frac{1}{2}, 1 + \\frac{1}{2} + \\frac{1}{3}, ..., H_N, ...\\\\) |\n",
    "| \\\\(\\sum_{N \\geq 0} N(H_N - 1)z^N = \\frac{z}{(1-z)^2}ln\\frac{1}{1-z}\\\\) | \\\\(0, 0, 1, 3(\\frac{1}{2}+\\frac{1}{3}), 4(\\frac{1}{2}+\\frac{1}{3}+\\frac{1}{4}), ... \\\\) |\n",
    "\n",
    "Table 1. Elementary generating function\n",
    "\n",
    "\n",
    "| OGF Operation  | Sequence  |                                    \n",
    "|:---------------|:----------|\n",
    "| \\\\(A(z) = \\sum_{n \\geq 0}z_n z^n\\\\) | \\\\(a_0, a_1, a_2, ..., a_n, ...\\\\) |\n",
    "| \\\\(B(z) = \\sum_{n \\geq 0}b_n z^n\\\\) | \\\\(b_0, b_1, b_2, .., b_n, ...\\\\) |\n",
    "| right shift<br> \\\\(zA(z) = \\sum{n \\geq 1}a_{n-1}z^n\\\\) | <br> \\\\(0, a_0, a_1, a_2, ..., a_{n-1}, ...\\\\) |\n",
    "| left shift<br> \\\\(\\frac{A(z)-a_0}{z} = \\sum_{n \\geq 0} a_{n+1}z^n\\\\) | \\\\(a_1, a_2, a_3, ..., a_{n+1}, ...\\\\) |\n",
    "| index multiply (differentiation)<br> \\\\(A'(z) = \\sum{n \\geq 0}(n+1)a_{n+1}z^n\\\\) | \\\\(a_1, 2a_2, ..., (n+1)a_{n+1}, ...\\\\) |\n",
    "| index divide (integration)<br> \\\\(\\int_{0}^{z} A(t)dt = \\sum_{n \\geq 1} \\frac{a_{n-1}}{n}z^n\\\\) | \\\\(0, a_0, \\frac{a_1}{2}, \\frac{a_2}{3}..., \\frac{a_{n-1}}{n}, ...\\\\) |\n",
    "| scaling<br> \\\\(A(\\lambda z) = \\sum_{n \\geq 0} {\\lambda}^n a_n z^n\\\\) | \\\\(a_0, \\lambda a_1, \\lambda^2 a_2, ..., \\lambda^n a_n, ...\\\\) |\n",
    "| addition<br> \\\\(A(z) + B(z) = \\sum_{n \\geq 0} (a_n + b_n)z^n\\\\) | \\\\(a_0+b_0, ..., a_n + b_n, ...\\\\) |\n",
    "| difference<br> \\\\((1-z)A(z) = a_0+\\sum_{n \\geq 1}(a_n-a_{n-1})z^n\\\\) | \\\\(a_0, a_1-a_0, ..., a_n-a_{n-1}, ...\\\\) |\n",
    "| convolution<br> \\\\(A(z)B(z) = \\sum_{n \\geq 0}\\big(\\sum_{0 \\le k \\leq n} a_kb_{n-k} \\big) z^n\\\\) | \\\\(a_0b_0, a_1b_0 + a_0b_1, ..., \\sum_{0 \\leq k \\leq n} a_kb_{n-k}, \\\\) |\n",
    "| partial sum<br> \\\\(\\frac{A(z)}{1-z} = \\sum_{n \\geq 0} \\big(\\sum_{0 \\leq k \\leq n} a_k \\big) z^n\\\\) | \\\\(a_1, a_1+a_2, ..., \\sum_{0 \\leq k \\leq n} a_k, ...\\\\) |\n",
    "\n",
    "Table 2. Operation on OGF\n",
    "\n",
    "\n",
    "### Theorem 3.1 (OGF)\n",
    "\n",
    "If two sequences \\\\(a_0, a_1, ..., a_k, ...\\\\) and \\\\(b_0, b_1, ..., b_k, ...\\\\) are represented by the OFSs \\\\(A(z) = \\sum_{k \\geq 0} a_k z^k\\\\) and \\\\(B(z) = \\sum_{b \\geq 0} b_k z^k\\\\), respectively, then the operation given in table 2 produce OGFs that represent the indicated sequences. In particular:\n",
    "\n",
    "$$\\eqalign{\n",
    "    A(z) + B(z) \\ \\text{is the OGF for} \\ a_0 + b_0, a_1 + b_1, a_2 + b_2, ...\\\\\n",
    "    zA(z) \\ \\text{is the OGF for} \\ 0, a_0, a_1, a_2, ...\\\\\n",
    "    A'(z) \\  \\text{is the OGF for} \\ a_1, 2a_2, 3a_3, ...\\\\\n",
    "    A(z)B(z) \\ \\text{is the OGF for} \\ a_0b_0, a_0b_1 + a_1b_0, a_0b_2 + a_1b_1 + a_2b_0, ...\n",
    "}$$\n",
    "\n",
    "\n",
    "**PROOF**: Most of these are elementary and can be verified by inspection. The *convolution* operation (and the *partial sum* special case) are easily proved by manipulating the order of summation:\n",
    "\n",
    "$$\\eqalign{\n",
    "    A(z)B(z) &= \\sum_{i \\geq 0} a_iz^i \\sum_{j \\geq 0} b_j z^j\\\\\n",
    "             &= \\sum_{i, j \\geq 0} a_ib_jz^{i+j}\n",
    "             &= \\sum_{n \\geq 0} \\bigl(\\sum_{0 \\leq k \\le n} a_k b_{n-k} \\bigr) z^n\n",
    "}$$\n",
    "\n",
    "Taking \\\\(B(z) = \\frac{a}{(1-z)}\\\\) in this formula gives the partial sum operation. The convolution operation plays a special role in generating function manipulations, as we shall see.\n",
    "\n",
    "**Corollary**: The OGF for the harmonic number is:\n",
    "\n",
    "$$\\sum_{N \\geq 1} H_Nz^N = \\frac{1}{1-z}ln\\frac{1}{1-z}$$\n",
    "\n",
    "**PROOF**: Start with \\\\(\\frac{1}{1-z}\\\\) (the OGF for 1, 1, ..., 1, ...), integrate (to get the OGF for 0, 1, 1/2, 1/2, ..., 1/k, ...), and multiply by \\\\(\\frac{1}{1-z}\\\\). Similar examples may be found in the relationships among the enttries in Table 1.\n",
    "\n",
    "\n",
    "## Exponential Generating Function (EGF)\n",
    "\n",
    "**Definition** Given a sequence \\\\(a_0, a_1, a_2, ..., a_k, ...,\\\\) the function:\n",
    "\n",
    "$$A(z) = \\sum_{k \\geq 0} a_k \\frac{z^k}{k!}$$\n",
    "\n",
    "is called the *exponential generating function (EGF)* of the sequence. We use the notation \\\\(k! \\lfloor z^k \\rfloor A(z)\\\\) to refer to the coefficient \\\\(a_k\\\\).\n",
    "\n",
    "Table 3 gives a number of elementary exponential generating functions and table 4 gives some of the basic manipulations of EGFs.\n",
    "\n",
    "| EGF   | Sequence  |                                    \n",
    "|:-----:|:----------|\n",
    "| \\\\(\\sum_{N \\geq 0} \\frac{z^N}{N!} = e^z\\\\) | \\\\(1, 1, 1, 1, ..., 1, ...\\\\) |\n",
    "| \\\\(\\sum_{N \\geq 1} \\frac{z^N}{(N-1)!} = ze^z\\\\) | \\\\(0, 1, 2, 3, 4, ..., N, ...\\\\) |\n",
    "| \\\\(\\frac{1}{2} \\sum_{N \\geq 2} \\frac{z^N}{(N-2)!} = \\frac{1}{2}z^2 e^z\\\\) | \\\\(0, 0, 1, 3, 6, 10, ..., {N \\choose 2}, ...\\\\) |\n",
    "| \\\\(\\frac{1}{M!} \\sum_{N \\geq M} \\frac{z^N}{(N-M)!} = \\frac{1}{M!} z^M e^z\\\\) | \\\\(0, ..., 0, 1, M+1, ..., {N \\choose M}, ...\\\\) |\n",
    "| \\\\(\\sum_{N \\geq 0} \\frac{1+(-1)^N}{2} \\frac{z^N}{N!} = \\frac{1}{2}(e^z + e^{-z})\\\\) | \\\\(1, 0, 1, 0, ..., 1, 0, ...\\\\) |\n",
    "| \\\\(\\sum_{N \\geq 0}\\frac{c^Nz^N}{N!} = e^{cz}\\\\) | \\\\(1, c, c^2, c^3, ..., c^N, ...\\\\) |\n",
    "| \\\\(\\sum_{N \\geq 0}\\frac{z^N}{(N+!)!} = \\frac{e^z-1}{z}\\\\) | \\\\(1, \\frac{1}{2}, \\frac{1}{3}, ..., \\frac{1}{N+1}, ...\\\\) |\n",
    "| \\\\(\\sum_{N \\geq 0}\\frac{N!z^N}{N!} = \\frac{1}{1-z}\\\\) | \\\\(1, 1, 2, 6, 24, ..., N!, ...\\\\) |\n",
    "\n",
    "Table 3. Elementary exponential generating functions\n",
    "\n",
    "| EGF Operation  | Sequence  |                                    \n",
    "|:---------------|:----------|\n",
    "| \\\\(A(z) = \\sum_{n \\geq 0}a_n \\frac{z^n}{n!}\\\\) | \\\\(a_0, a_1, a_2, ..., a_n, ...\\\\) |\n",
    "| \\\\(B(z) = \\sum_{n \\geq 0}b_n \\frac{z^n}{n!}\\\\) | \\\\(b_0, b_1, b_2, .., b_n, ...\\\\) |\n",
    "| right shift (integration)<br> \\\\(\\int_0^z A(t)d(t) = \\sum{n \\geq 1}a_{n-1}\\frac{z^n}{n!}\\\\) | <br> \\\\(0, a_0, a_1, a_2, ..., a_{n-1}, ...\\\\) |\n",
    "| left shift (differentiation)<br> \\\\(A'(z)= \\sum_{n \\geq 0} a_{n+1} \\frac{z^n}{n!}\\\\) | \\\\(a_1, a_2, a_3, ..., a_{n+1}, ...\\\\) |\n",
    "| index multiply<br> \\\\(zA(z) = \\sum{n \\geq 0}na_{n-1}\\frac{z^n}{n!}\\\\) | \\\\(0, a_0, 2a_1, 3_a, ..., na_{n-1}, ...\\\\) |\n",
    "| index divide<br> \\\\((A(z) - A(0)/z = \\sum_{n \\geq 1}\\frac{a_{n+1}}{n+1} \\frac{z^n}{n!})\\\\) | \\\\(a_1, \\frac{a_2}{2}, \\frac{a_3}{3}, ..., \\frac{a_{n+1}}{n+1}, ...\\\\) |\n",
    "| addition<br> \\\\(A(z) + B(z) = \\sum_{n \\geq 0} (a_n + b_n)\\frac{z^n}{n!}\\\\) | \\\\(a_0+b_0, ..., a_n + b_n, ...\\\\) |\n",
    "| difference<br> \\\\(A'(z)-A(z) = \\sum_{n \\geq 0}(a_{n+1}-a_n)\\frac{z^n}{n!}\\\\) | \\\\(a_0+b_0, ..., a_n+b_n, ...\\\\) |\n",
    "| binomial convolution<br> \\\\(A(z)B(z) = \\sum_{n \\geq 0}\\big(\\sum_{0 \\le k \\leq n} a_kb_{n-k} \\big) \\frac{z^n}{n!}\\\\) | \\\\(a_0b_0, a_1b_0 + a_0b_1, ..., \\sum_{0 \\leq k \\leq n} {n \\choose k} a_kb_{n-k}, \\\\) |\n",
    "| binomial sum<br> \\\\(e^z A(z) = \\sum_{n \\geq 0} \\big(\\sum_{0 \\leq k \\leq n} {n \\choose k} a_k \\big) \\frac{z^n}{n!}\\\\) | \\\\(a_0, a_0 + a_1, ..., \\sum_{0 \\leq k \\leq n} {n \\choose k} a_k, ...\\\\) |\n",
    "\n",
    "Table 4. Operation on EGF\n",
    "\n",
    "\n",
    "### Theorem 3.2 (EGF operations)\n",
    "\n",
    "If two sequences \\\\(a_0, a_1, ..., a_k, ...\\\\) and \\\\(b_0, b_1, ..., b_k, ...\\\\) are represented by the EGFs \\\\(A(z) = \\sum_{k \\geq 0} \\frac{a_k z^k}{k!}\\\\) and \\\\(B(z) = \\sum_{k \\geq 0} \\frac{b_k z^k}{k!}\\\\), respectively, then the operations given in Table 4 produce EGFs that represent the indicated sequences. In particular,\n",
    "\n",
    "$$\\eqalign{\n",
    "    A(z) + B(z) \\ \\text{is the EGF for} \\ a_0 + b_0, a_1 + b_1, a_2 + b_2, ...\\\\\n",
    "    A'(z) \\ \\text{is the EGF for} \\ a_1, a_2, a_3 ...\\\\\n",
    "    zA(z) \\  \\text{is the EGF for} \\ 0, a_0, 2a_1, 3a_2, ...\\\\\n",
    "    A(z)B(z) \\ \\text{is the EGF for} \\ a_0b_0, a_0b_1 + a_1b_0, a_0b_2 + a_1b_1 + a_2b_0, ...\n",
    "}$$\n",
    "\n",
    "\n",
    "**PROOF**: As for theorem 3.1, these are elementary and can be verified by inspection woth possible exception of binomial convolution, which is easily verified with OGF convolution:\n",
    "\n",
    "$$\\eqalign{\n",
    "    A(z)B(z) &= \\sum_{n \\geq 0} \\sum_{0 \\leq k \\leq n} \\frac{a_k}{k!} \\frac{b_{n-k}}{(n-k)!}z^n\\\\\n",
    "             &= \\sum_{n \\geq 0} \\sum_{0 \\leq k \\leq n} {n \\choose k} a_k b_{n-k} \\frac{z^n}{n!}\n",
    "}$$\n",
    "\n",
    "we can automatically convert from the OGF for a sequence to the EGF for the same sequence, and vice versa by using **Laplace transformation**.\n",
    "\n",
    "\n",
    "## Generating Function Solution of Recurrences\n",
    "\n"
   ]
  },
  {
   "cell_type": "code",
   "execution_count": null,
   "metadata": {},
   "outputs": [],
   "source": []
  }
 ],
 "metadata": {
  "kernelspec": {
   "display_name": "Python 3",
   "language": "python",
   "name": "python3"
  },
  "language_info": {
   "codemirror_mode": {
    "name": "ipython",
    "version": 3
   },
   "file_extension": ".py",
   "mimetype": "text/x-python",
   "name": "python",
   "nbconvert_exporter": "python",
   "pygments_lexer": "ipython3",
   "version": "3.6.4"
  }
 },
 "nbformat": 4,
 "nbformat_minor": 2
}
